toLabeled with guard, not big step

lio.v
@@ -54,7 +54,9 @@ Inductive t : Set :=  (*r term *)
  | t_GetClearance : t (*r get current clearance *)
  | t_LabelOf (t5:t) (*r get label of value *)
  | t_Label (t5:t) (t':t) (*r label *)
- | t_UnLabel (t5:t) (*r unlabel *).
+ | t_UnLabel (t5:t) (*r unlabel *)
+ | t_ToLabeled (t1:t) (t2:t) (*r execute sensitive computation *)
+ | t_MkToLabeledTCB (l_5:t) (c:t) (l1:t) (t5:t) (*r trusted primitive that restores computation *).
 
 Definition G : Set := list (termvar*T).
 
@@ -95,6 +97,8 @@ Definition is_l_of_t (t_6:t) : Prop :=
   | (t_LabelOf t5) => False
   | (t_Label t5 t') => False
   | (t_UnLabel t5) => False
+  | (t_ToLabeled t1 t2) => False
+  | (t_MkToLabeledTCB l_5 c l1 t5) => False
 end.
 
 Fixpoint is_t_of_t (t_6:t) : Prop :=
@@ -124,6 +128,8 @@ Fixpoint is_t_of_t (t_6:t) : Prop :=
   | (t_LabelOf t5) => ((is_t_of_t t5))
   | (t_Label t5 t') => ((is_t_of_t t5) /\ (is_t_of_t t'))
   | (t_UnLabel t5) => ((is_t_of_t t5))
+  | (t_ToLabeled t1 t2) => ((is_t_of_t t1) /\ (is_t_of_t t2))
+  | (t_MkToLabeledTCB l_5 c l1 t5) => ((is_l_of_t l_5) /\ (is_l_of_t c) /\ (is_l_of_t l1) /\ (is_t_of_t t5))
 end.
 
 Definition is_v_of_t (t_6:t) : Prop :=
@@ -153,6 +159,8 @@ Definition is_v_of_t (t_6:t) : Prop :=
   | (t_LabelOf t5) => False
   | (t_Label t5 t') => False
   | (t_UnLabel t5) => False
+  | (t_ToLabeled t1 t2) => False
+  | (t_MkToLabeledTCB l_5 c l1 t5) => False
 end.
 
 Definition is_m_of_m (m5:m) : Prop :=
@@ -204,6 +212,8 @@ Fixpoint fv_t (t_6:t) : list termvar :=
   | (t_LabelOf t5) => ((fv_t t5))
   | (t_Label t5 t') => (app (fv_t t5) (fv_t t'))
   | (t_UnLabel t5) => ((fv_t t5))
+  | (t_ToLabeled t1 t2) => (app (fv_t t1) (fv_t t2))
+  | (t_MkToLabeledTCB l_5 c l1 t5) => ((fv_t t5))
 end.
 
 Definition fv_m (m5:m) : list termvar :=
@@ -240,6 +250,8 @@ Fixpoint tsubst_t (t_6:t) (x5:termvar) (t__7:t) {struct t__7} : t :=
   | (t_LabelOf t5) => t_LabelOf (tsubst_t t_6 x5 t5)
   | (t_Label t5 t') => t_Label (tsubst_t t_6 x5 t5) (tsubst_t t_6 x5 t')
   | (t_UnLabel t5) => t_UnLabel (tsubst_t t_6 x5 t5)
+  | (t_ToLabeled t1 t2) => t_ToLabeled (tsubst_t t_6 x5 t1) (tsubst_t t_6 x5 t2)
+  | (t_MkToLabeledTCB l_5 c l1 t5) => t_MkToLabeledTCB l_5 c l1 (tsubst_t t_6 x5 t5)
 end.
 
 Definition tsubst_m (t_6:t) (x5:termvar) (m5:m) : m :=
@@ -347,7 +359,25 @@ Inductive GtT : G -> t -> T -> Prop :=    (* defn GtT *)
  | GtT_unlabel : forall (G5:G) (t5:t) (T5:T),
      is_t_of_t t5 ->
      GtT G5 t5 (T_TLabeled T5) ->
-     GtT G5 (t_UnLabel t5) (T_TLIO T5).
+     GtT G5 (t_UnLabel t5) (T_TLIO T5)
+ | GtT_toLabeled : forall (G5:G) (t1 t2:t) (T5:T),
+     is_t_of_t t1 ->
+     is_t_of_t t2 ->
+     GtT G5 t1 T_TLabel ->
+     GtT G5 t2 (T_TLIO T5) ->
+     GtT G5 (t_ToLabeled t1 t2) (T_TLIO  (T_TLabeled T5) )
+ | GtT_mkToLabeledTCB : forall (G5:G) (t5:t) (T5:T) (l_5 c l1:t),
+     is_l_of_t l_5 ->
+     is_l_of_t l1 ->
+     is_t_of_t t5 ->
+     is_l_of_t l_5 ->
+     is_l_of_t c ->
+     is_l_of_t l1 ->
+     GtT G5 l_5 T_TLabel ->
+     GtT G5 c T_TLabel ->
+     GtT G5 l1 T_TLabel ->
+     GtT G5 t5 T5 ->
+     GtT G5 (t_MkToLabeledTCB l_5 c l1 t5) (T_TLIO  (T_TLabeled T5) ).
 (** definitions *)
 
 (* defns Jpop *)
@@ -573,6 +603,25 @@ Inductive lio_reduce : m -> m -> Prop :=    (* defn lio_reduce *)
      pure_reduce (t_Join l_5 l1) l2 ->
      pure_reduce (t_CanFlowTo l2 c) t_VTrue ->
      lio_reduce (m_Config l_5 c (t_UnLabel  (t_VLabeled l1 t2) )) (m_Config l2 c (t_Return t2))
+ | LIO_toLabeled : forall (t5:t) (x:termvar) (l1 l_5 c:t),
+     is_l_of_t l_5 ->
+     is_l_of_t l1 ->
+     is_t_of_t t5 ->
+     is_l_of_t l1 ->
+     is_l_of_t l_5 ->
+     is_l_of_t c ->
+     pure_reduce (t_CanFlowTo l_5 l1) t_VTrue ->
+     pure_reduce (t_CanFlowTo l1 c) t_VTrue ->
+     lio_reduce (m_Config l_5 c (t_ToLabeled l1 t5)) (m_Config l_5 c (t_Bind t5  (t_VAbs x (t_MkToLabeledTCB l_5 c l1 (t_Var x))) ))
+ | LIO_mkToLabeledTCB : forall (c l' c' v5 l1 l_5:t),
+     is_l_of_t l_5 ->
+     is_l_of_t l' ->
+     is_l_of_t l1 ->
+     is_v_of_t v5 ->
+     is_l_of_t l1 ->
+     is_l_of_t l_5 ->
+     pure_reduce (t_CanFlowTo l_5 l1) t_VTrue ->
+     lio_reduce (m_Config l_5 c (t_MkToLabeledTCB l' c' l1 v5)) (m_Config l' c' (t_Label l1 v5))
 with lio_multi_reduce : m -> m -> Prop :=    (* defn lio_multi_reduce *)
  | lio_multi_refl : forall (l5 c t5:t),
      is_l_of_t l5 ->
@@ -735,6 +784,15 @@ Inductive term_erasure : t -> t -> t -> Prop :=    (* defn term_erasure *)
      is_t_of_t t' ->
      term_erasure l5 t5 t' ->
      term_erasure l5 (t_UnLabel t5) (t_UnLabel t')
+ | Te_toLabeled : forall (l5 t1 t2 t1' t2':t),
+     is_l_of_t l5 ->
+     is_t_of_t t1 ->
+     is_t_of_t t2 ->
+     is_t_of_t t1' ->
+     is_t_of_t t2' ->
+     term_erasure l5 t1 t1' ->
+     term_erasure l5 t2 t2' ->
+     term_erasure l5 (t_ToLabeled t1 t2) (t_ToLabeled t1' t2')
 with lio_erasure : t -> m -> m -> Prop :=    (* defn lio_erasure *)
  | Ce_conf : forall (c1 t1 t1' l1 l_5:t),
      is_l_of_t l_5 ->
@@ -842,9 +900,8 @@ Tactic Notation "lio_reduce_cases" tactic(first) ident(c) :=
   | Case_aux c "LIO_label"
   | Case_aux c "LIO_unlabelCtx"
   | Case_aux c "LIO_unlabel"
-(*
-  | Case_aux c "LIO_toLabeledCtx"
-  | Case_aux c "LIO_toLabeled" *) ].
+  | Case_aux c "LIO_toLabeled"
+  | Case_aux c "LIO_mkToLabeledTCB" ].
 
 
 
